pulse/src/checker/Pulse.Syntax.Pure.fst
@@ -368,7 +368,7 @@ let tm_add_inv (is iname:R.term) : R.term =
 let tm_later (p:term) : term =
   let h = R.pack_ln (R.Tv_FVar (R.pack_fv later_lid)) in
   R.mk_app h [ex p]
-let tm_full_perm = tm_constant (R.C_Real "1.0")
+let tm_full_perm = tm_constant (R.C_Real (FStar.RealLiteral.of_int 1))
 
 
 let is_view_of (tv:term_view) (t:term) : prop =
